src/axiomatic/TsoSimLocal.v
@@ -381,29 +381,34 @@ Proof.
   - inv H1. ss. subst. eapply FWDN. econs; eauto. econs; eauto with tso.
 Qed.
 
-Definition sim_local_vpn ex :=
+Definition sim_local_vpn ex loc :=
   (⦗ex.(Execution.label_is) Label.is_kinda_read⦘ ⨾
    Execution.po) ∪
 
-  (⦗ex.(Execution.label_is) Label.is_access⦘ ⨾
+  (⦗ex.(Execution.label_is) (Label.is_writing_cl loc)⦘ ⨾
+   Execution.po) ∪
+
+  (⦗ex.(Execution.label_is) (Label.is_access)⦘ ⨾
    Execution.po ⨾
    (⦗ex.(Execution.label_is) (Label.is_barrier_c Barrier.is_mfence)⦘ ∪
     ⦗ex.(Execution.label_is) (Label.is_barrier_c Barrier.is_sfence)⦘) ⨾
    Execution.po).
 
-Lemma sim_local_vpn_step ex:
-  sim_local_vpn ex =
-  (sim_local_vpn ex ∪
+Lemma sim_local_vpn_step ex loc:
+  sim_local_vpn ex loc =
+  (sim_local_vpn ex loc ∪
    ((⦗ex.(Execution.label_is) Label.is_kinda_read⦘) ∪
 
-   (⦗ex.(Execution.label_is) Label.is_access⦘ ⨾
+    (⦗ex.(Execution.label_is) (Label.is_writing_cl loc)⦘) ∪
+
+    (⦗ex.(Execution.label_is) (Label.is_access)⦘ ⨾
      Execution.po ⨾
      (⦗ex.(Execution.label_is) (Label.is_barrier_c Barrier.is_mfence)⦘ ∪
       ⦗ex.(Execution.label_is) (Label.is_barrier_c Barrier.is_sfence)⦘)))) ⨾
   Execution.po_adj.
 Proof.
   unfold sim_local_vpn. rewrite ? (union_seq' Execution.po_adj), ? seq_assoc, ? union_assoc.
-  rewrite Execution.po_po_adj at 1 3.
+  rewrite Execution.po_po_adj at 1 2 4.
   rewrite (clos_refl_union Execution.po), union_seq, eq_seq.
   rewrite ? (seq_union' (Execution.po ⨾ Execution.po_adj) Execution.po_adj), ? seq_assoc, ? union_assoc.
   funext. i. funext. i. propext. econs; i.
@@ -423,7 +428,7 @@ Definition sim_local_lper ex loc :=
    ⦗ex.(Execution.label_is) (Label.is_flushing_cl loc)⦘ ⨾
    Execution.po) ∪
 
-  ((sim_local_coh ex loc ∪ sim_local_vpn ex) ⨾
+  (sim_local_vpn ex loc ⨾
    ⦗ex.(Execution.label_is) (Label.is_flushopting_cl loc)⦘ ⨾
    Execution.po).
 
@@ -432,7 +437,7 @@ Lemma sim_local_lper_step ex loc:
   (sim_local_lper ex loc ∪
    ((sim_local_vwn ex ⨾
      ⦗ex.(Execution.label_is) (Label.is_flushing_cl loc)⦘) ∪
-    ((sim_local_coh ex loc ∪ sim_local_vpn ex) ⨾
+    (sim_local_vpn ex loc ⨾
      ⦗ex.(Execution.label_is) (Label.is_flushopting_cl loc)⦘))) ⨾
   Execution.po_adj.
 Proof.
